Regex/Data/Array/Basic.lean
@@ -1,0 +1,21 @@
+import Std.Data.Nat.Lemmas
+
+namespace Array
+
+/-- get head element and array without head element -/
+def head? (a : Array α) : Option (α × Array α) :=
+  match a.data with
+  | [] => none
+  | List.cons head tail => some (head, ⟨tail⟩)
+
+/-- get last element and array without last element -/
+def pop? (a : Array α) : Option (α × Array α) :=
+  if h : 0 < a.data.length
+  then some ((a.data.get ⟨a.data.length - 1, Nat.sub_lt h Nat.one_pos⟩), a.pop)
+  else none
+
+/-- get last element of array -/
+def last? (a : Array α) : Option α :=
+  if h : 0 < a.data.length
+  then a.data.get ⟨a.data.length - 1, Nat.sub_lt h Nat.one_pos⟩
+  else none
