Regex/Data/List/Lemmas.lean
@@ -1,0 +1,61 @@
+import Std.Data.Nat.Lemmas
+import Std.Data.Fin.Lemmas
+import Std.Data.Int.Lemmas
+import Std.Data.List.Basic
+import Std.Data.List.Lemmas
+
+import Regex.Data.Nat.Basic
+
+namespace List
+
+theorem singleton_val_of (a : α) (arr : List α) (h1 : arr = [a]) (h2 : 0 < List.length arr)
+    : List.get arr ⟨0, h2⟩ = a  := by
+  unfold List.get
+  split <;> simp_all
+  unfold List.get
+  split <;> simp_all
+
+theorem singleton_val (a : α) (h : 0 < List.length [a])
+    : List.get [a] ⟨0, h⟩ = a  := by
+  simp [List.singleton_val_of a [a] (by simp) h]
+
+theorem get_of_fun_eq {l1 l2 : List α} {f : List α → List α} (h : f l1 = f l2)
+  (n : Fin (f l1).length) : (f l1).get n = (f l2).get ⟨n, h ▸ n.2⟩ :=
+  List.get_of_eq h n
+
+theorem eq_of_dropLast_eq_last_eq {l1 l2 : List α} (hd : List.dropLast l1 = List.dropLast l2)
+  (hl1 : l1.length - 1 < l1.length) (hl2 : l2.length - 1 < l2.length)
+  (heq : List.get l1 ⟨l1.length - 1, hl1⟩  = List.get l2 ⟨l2.length - 1, hl2⟩) : l1 = l2 :=
+  have hdl : l1.dropLast.length = l2.dropLast.length := by rw [hd]
+  have hn1 : 0 < l1.length := Nat.zero_lt_of_lt hl1
+  have hn2 : 0 < l2.length := Nat.zero_lt_of_lt hl2
+  have hl : l1.length = l2.length := by
+    have h1 : l1.dropLast.length = l1.length - 1 := List.length_dropLast l1
+    have h2 : l2.dropLast.length = l2.length - 1 := List.length_dropLast l2
+    rw [hdl, h2] at h1
+    simp [Nat.pred_inj hn1 hn2 h1.symm]
+  List.ext_get hl fun n h1 h2 =>
+    if hx1 : n < l1.dropLast.length then by
+      have hx2 : n < l2.dropLast.length := Nat.lt_of_lt_of_eq hx1 hdl
+      have hy1 : l1.dropLast.get ⟨n, hx1⟩ = l1.get ⟨n, h1⟩ := List.get_dropLast l1 ⟨n, hx1⟩
+      have hy2 : l2.dropLast.get ⟨n, hx2⟩ = l2.get ⟨n, h2⟩ := List.get_dropLast l2 ⟨n, hx2⟩
+      have hy3 : l1.dropLast.get ⟨n, hx1⟩ = l2.dropLast.get ⟨n, hx2⟩ := List.get_of_fun_eq hd ⟨n, hx1⟩
+      rw [hy3, hy2] at hy1
+      rw [hy1]
+    else by
+      rw [List.length_dropLast l1] at hx1
+      simp [Nat.le_of_not_gt] at hx1
+      have hn1 : n = l1.length - 1 := by
+        simp [Nat.eq_pred_of_le_of_lt_succ hn1 hx1 h1]
+        rfl
+      have hn2 : n = l2.length - 1 := by
+        have hx2 : List.length l2 - 1 ≤ n := by
+          rw [hl] at hx1
+          simp [hx1]
+        simp_all [Nat.eq_pred_of_le_of_lt_succ hn2 hx2 h2]
+      simp [← hn1, ← hn2] at heq
+      simp [heq]
+
+theorem get_last_of_concat {l : List α} (h : (l ++ [last]).length - 1 < (l ++ [last]).length)
+    : List.get (l ++ [last]) ⟨(l ++ [last]).length - 1, h⟩ = last  := by
+  simp [List.get_last _]
