Regex/Data/Nat/Basic.lean
@@ -14,3 +14,11 @@ theorem le_lt_sub_lt {i j n : Nat} (h1 : i ≤ j) (h2 : j < n) :  j - i < n := b
   have hy : n ≤ i + n := Nat.le_add_left n i
   have hx : j < i + n := Nat.lt_of_lt_of_le h2 hy
   simp [Nat.sub_lt_left_of_lt_add h1 hx]
+
+theorem eq_pred_of_le_of_lt_succ {n m : Nat} (h0 : 0 < n) (h1 : n.pred ≤ m) (h2 : m < n)
+    : m = n.pred := by
+  have h : m ≤ n.pred := by
+    have : n = Nat.succ (n.pred) := by cases h0 <;> rfl
+    rw [this] at h2
+    simp [Nat.le_of_lt_succ h2]
+  simp [Nat.le_antisymm h1 h]
