Regex/Data/UInt/Basic.lean
@@ -13,6 +13,15 @@ theorem add_def {a b : UInt32} : UInt32.add a b = a + b := rfl
 
 theorem sub_def {a b : UInt32} : UInt32.sub a b = a - b := rfl
 
+theorem eq_of_val_eq : ∀ {i j : UInt32}, Eq i.val j.val → Eq i j
+  | ⟨_, _⟩, ⟨_, _⟩, rfl => rfl
+
+theorem val_eq_of_eq {i j : UInt32} (h : Eq i j) : Eq i.val j.val :=
+  h ▸ rfl
+
+theorem val_ne_of_ne {c d : UInt32} (h : Not (Eq c d)) : Not (Eq c.val d.val) :=
+  fun h' => absurd (eq_of_val_eq h') h
+
 theorem one_le_of_lt {c1 c2 : UInt32} (h : c1 < c2) : 1 ≤ c2 :=
   Nat.zero_lt_of_lt h
 
@@ -26,12 +35,6 @@ theorem toNat_toUInt_eq (u : UInt32) : u.toNat.toUInt32 = u := by
 theorem ofNat_eq (n : Nat) (h : n < UInt32.size) : (UInt32.ofNat n).val = ⟨n, h⟩ := by
   unfold UInt32.ofNat
   simp [Fin.ofNat_eq n h]
-
-theorem eq_of_val_eq : ∀ {i j : UInt32}, Eq i.val j.val → Eq i j
-  | ⟨_, _⟩, ⟨_, _⟩, rfl => rfl
-
-theorem val_eq_of_eq {i j : UInt32} (h : Eq i j) : Eq i.val j.val :=
-  h ▸ rfl
 
 theorem ofNat_add_ofNat (n m : Nat) (hn : n < UInt32.size) (hm : m < UInt32.size)
   (hnm : n + m < UInt32.size) : (UInt32.ofNat n) + (UInt32.ofNat m) = UInt32.ofNat (n + m) := by
