Regex/Interval/Basic.lean
@@ -1,0 +1,140 @@
+import Init.Data.Ord
+import Std.Logic
+import Std.Data.Nat.Lemmas
+import Std.Data.Fin.Lemmas
+import Std.Data.Int.Lemmas
+import Std.Data.List.Basic
+import Regex.Utils
+import Regex.Data.Array.Basic
+import Regex.Bound
+import Regex.Data.UInt.Basic
+import Regex.Data.Char.Basic
+
+/-!
+## IntervalSet
+
+This file contains an implementation of interval sets (`IntervalSet`),
+a sorted set of non-overlapping ranges (`Range`).
+-/
+
+/-- A closed range bounded inclusively below and above (`start..end`). -/
+structure Range (α : Type u) [Ord α] [LE α] [Bound α] where
+  start: α
+  «end»: α
+  isLe: start ≤ «end»
+deriving Repr, DecidableEq
+
+instance (α : Type u) [Ord α] [LE α] [LT α] [Bound α]: LT $ Range α where
+  lt r1 r2 := r1.end < r2.start
+
+instance : ToString $ Range Char where
+  toString s := s!"{s.start} {s.end}"
+
+instance : Inhabited $ Range Char where
+  default := ⟨default, default, of_decide_eq_true rfl⟩
+
+namespace Range
+
+/-- ranges `r1` and `r2` are non overlapping when they are sorted and
+    they are not overlapping or adjacent -/
+def nonOverlapping {α : Type u} [Ord α] [LE α] [LT α] [Bound α] [HSub α α Nat]
+    (r1 r2 : Range α) : Prop :=
+   1 < ((r2.start - r1.end) : Nat)
+
+instance {α : Type u} [Ord α] [LE α] [LT α] [Bound α] [HSub α α Nat]
+    (r1 r2 : Range α) : Decidable (Range.nonOverlapping r1 r2) :=
+  inferInstanceAs (Decidable (LT.lt 1 ((r2.start - r1.end) : Nat)))
+
+def intersection {α : Type u} [Ord α]
+    [LT α] [LE α] [Bound α] [(a b : α) → Decidable (a ≤ b)]
+    (r1 r2 : Range  α) : Option $ Range α :=
+  let lower := if r1.start ≤ r2.start then r2.start else r1.start
+  let upper := if r1.«end» ≤ r2.«end» then r1.«end» else r2.«end»
+  if h : lower ≤ upper then some ⟨lower, upper, h⟩
+  else none
+
+def Char.sub (c₁ c₂ : Char) := c₁.toNat - c₂.toNat
+
+instance : HSub Char Char Nat where
+  hSub := Char.sub
+
+theorem Char.sub_def {a b : Char} : Char.sub a b = a - b := rfl
+
+def negate (r1 r2 : Range Char) (h : nonOverlapping r1 r2) : Range Char :=
+  ⟨Bound.increment r1.end, Bound.decrement r2.start, by
+    unfold nonOverlapping at h
+    unfold Bound.increment
+    unfold Bound.decrement
+    unfold instBoundCharInstOrdCharInstLEChar
+    simp_all
+    have h : 1 + r1.end.toNat < r2.start.toNat := by simp [Nat.add_lt_of_lt_sub h]
+    simp [Bound.Char.incr_le_decr h]⟩
+
+end Range
+
+namespace Ranges
+
+def unique (ranges: Array (Range Char)) : Array (Range Char) :=
+  match ranges.data with
+  | [] => #[]
+  | [r] => #[r]
+  | head :: tail  =>
+    let (_, unique) := tail |> List.foldl (init := (head, #[head]))
+      (fun (prev, unique) r =>
+        if prev = r then (r, unique)
+        else (r, unique.push r))
+    unique
+
+/-- a list of ranges is non overlapping when ranges are sorted
+    and no ranges are overlapping or adjacent -/
+def dataIsNonOverlapping {α : Type u} [Ord α] [LT α] [LE α] [Bound α] [HSub α α Nat]
+    (ranges: List (Range α)) : Prop :=
+  match ranges with
+  | [] => true
+  | [_] => true
+  | head :: tail  => List.Chain (Range.nonOverlapping) head tail
+
+/-- an array of ranges is non overlapping when `ranges.data` is non overlapping -/
+def nonOverlapping {α : Type u} [Ord α] [LT α] [LE α] [Bound α] [HSub α α Nat]
+    (ranges: Array (Range α)) : Prop :=
+  dataIsNonOverlapping ranges.data
+
+end Ranges
+
+/-- A sorted set of non-overlapping ranges. -/
+structure IntervalSet (α : Type u) [Ord α] [LT α] [LE α] [Bound α] [HSub α α Nat]
+    [(a b : α) → Decidable (a < b)] [(a b : α) → Decidable (a = b)] where
+  ranges: Array (Range α)
+  isNonOverlapping: Ranges.nonOverlapping ranges
+deriving Repr
+
+instance : ToString $ IntervalSet Char where
+  toString s := s!"{s.ranges}"
+
+namespace Interval
+
+/-- last element of array `ranges` is non overlapping with range `next` -/
+def nonOverlappingWithLast (ranges : Array $ Range Char) (next : Option (Range Char)) : Prop :=
+  match ranges.last?, next with
+  | some last, some next => Range.nonOverlapping last next
+  | none , some _ => true
+  | none, none => true
+  | some _, none => false
+
+/-- Accumulator for loop in canonicalize -/
+structure Acc where
+  next : Option (Range Char)
+  set : IntervalSet Char
+  nonOverlapping : nonOverlappingWithLast set.ranges next
+
+def Acc.push (acc : Acc) (next : Range Char)
+  (h : Ranges.nonOverlapping (Array.push acc.set.ranges next)) : IntervalSet Char :=
+  ⟨acc.set.ranges.push next, h⟩
+
+/-- is `next.start` equal to `n.start` -/
+def is_start_eq (next : Option (Range Char)) (n : Range Char) : Prop :=
+  match next with
+  | some next  => next.start = n.start
+  | _ => true
+
+end Interval
