Regex/Interval/Intersection.lean
@@ -1,0 +1,171 @@
+import Init.Data.Ord
+import Regex.Utils
+import Regex.Bound
+import Regex.Interval.Basic
+import Regex.Interval.Lemmas
+
+/-!
+## IntervalSet
+
+IntervalSet operations like `Interval.intersection`
+-/
+
+namespace Interval
+
+def Acc.with_none (acc : Acc) (n : Range Char) (h : acc.next.isNone) : Acc :=
+  {acc with next := n, nonOverlapping := nonOverlappingWithLast_of_none acc n h}
+
+def Acc.with_next (acc : Acc) (n : Range Char) (h1 : is_start_eq acc.next n) : Acc :=
+  {acc with next := n, nonOverlapping := nonOverlappingWithLast_of_val acc n h1}
+
+def Acc.with_next_set (acc : Acc) (l r : Range Char) (h1 : Range.nonOverlapping l r)
+  (h2 : acc.next = some l) : Acc :=
+  match hm : acc.set.ranges.last? with
+  | some _ =>
+    have : Ranges.nonOverlapping (Array.push acc.set.ranges l) :=
+              nonOverlapping_of_push acc l hm h2
+    {acc with next := r,
+              set := Acc.push acc l this,
+              nonOverlapping := nonOverlappingWithLast_of_push acc h2 this h1}
+  | none =>
+    {acc with next := r, set := Interval.singleton l,
+              nonOverlapping := nonOverlappingWithLast_of_singleton l r h1}
+
+instance : Inhabited Acc :=
+  ⟨⟨none, default, nonOverlappingWithLast_of_empty default none
+                        (Array.default_size_zero default (by simp))⟩⟩
+
+/-- Converts `ranges` into `IntervalSet` with canonical ordering.  -/
+def canonicalize (ranges : Array (Range Char)) : IntervalSet Char :=
+  let _ranges := Array.qsort ranges
+                  (fun a b => a.start = b.start && a.end < b.end || a.start < b.start)
+  let _ranges := Ranges.unique _ranges
+
+  let init : Acc := default
+  let acc := _ranges |> Array.foldl (init := init) (fun acc r =>
+    match hm : acc.next with
+    | some l =>
+      if h1 : (r.start.toNat - l.end.toNat) = 1 then  -- [a-bc-d] => [a-d]
+        let next : Range Char := ⟨l.start, r.end, by
+            have hx : l.end < r.start := by simp [Char.succ_lt h1]
+            have hy : l.end ≤ r.start := by simp [Char.lt_le hx]
+            have hz : l.start ≤ r.start := by simp [Char.le_trans l.isLe hy]
+            simp [Char.le_trans hz r.isLe]
+        ⟩
+        Acc.with_next acc next (is_start_eq_of_val acc.next next hm (by simp))
+      else if h2 : l.start = r.start then -- [a-ca-d] => [a-d]
+        if l.end < r.end
+        then
+          let next : Range Char := ⟨l.start, r.end, by
+            have hx : l.start ≤ r.start := by simp [Char.eq_le h2]
+            simp [Char.le_trans hx r.isLe]
+          ⟩
+          Acc.with_next acc next (is_start_eq_of_val acc.next next hm (by simp))
+        else acc -- r.start = l.start ∧ r.end < l.end
+      else if h2 : r.start < l.end then -- [a-cb-d] => [a-d]
+        if r.end ≤ l.end -- [a-eb-d] => [a-e]
+        then acc
+        else if h : l.start < r.start -- [a-cb-d] => [a-d]
+        then
+          let next : Range Char := ⟨l.start, r.end, by
+            have hx : l.start ≤ r.start := by simp [Char.lt_le h]
+            simp [Char.le_trans hx r.isLe]
+          ⟩
+          Acc.with_next acc next (is_start_eq_of_val acc.next next hm (by simp))
+        else -- ¬l.start = r.start ∧ ¬l.start < r.start => r.start < l.start
+          panic s!"internal error: array not sorted at {l} {r}"
+      else if l.end = r.start && r.start = r.end then acc
+      else if h3 : l.end = r.start then -- [a-bb-c] => [a-c]
+        let next : Range Char := ⟨l.start, r.end, by
+          have hx : l.end ≤ r.start := by simp [Char.eq_le h3]
+          have hy : l.start ≤ r.start := by simp [Char.le_trans l.isLe hx]
+          simp [Char.le_trans hy r.isLe]
+        ⟩
+        Acc.with_next acc next (is_start_eq_of_val acc.next next hm (by simp))
+      else if r.start < l.start then panic s!"internal error: array not sorted at {l} {r}"
+      else -- [a-eg-h] => [a-eg-h]
+        have : Range.nonOverlapping l r := isNonOverlapping l r h1 h2 h3
+        Acc.with_next_set acc l r this hm
+    | none => Acc.with_none acc r (by unfold Option.isNone; simp_all [hm]))
+
+  let intervalSet :=
+    match hm : acc.next with
+    | some v =>
+        match hn : acc.set.ranges.last? with
+        | some _ => Acc.push acc v (nonOverlapping_of_push acc v hn (by simp[hm]; simp_all))
+        | none => Interval.singleton v
+    | none => acc.set
+
+  intervalSet
+
+/-- Negate a interval set. -/
+def negate (interval : IntervalSet Char) : IntervalSet Char :=
+  if interval.ranges.size = 0
+  then
+    singleton ⟨(Bound.min_value : Char), Bound.max_value, Bound.min_value_le_max_value⟩
+  else
+    let ranges : Array (Range Char) :=
+      Array.mapIdx interval.ranges  (fun i x => (i, x))
+      |> Array.map (fun (i, y) =>
+        if h : 0 < i.val
+        then
+          let x := interval.ranges.get ⟨i - 1, Fin.pred h⟩
+          let y := interval.ranges.get i
+          Range.negate x y
+            (Interval.nonOverlapping_of_pred interval.ranges i x y h
+                        (by simp) (by simp) interval.isNonOverlapping)
+        else
+          if Bound.min_value < y.start
+          then ⟨Bound.min_value, Bound.decrement y.start, by
+              simp [Bound.min_value_le_decrement y.start]
+            ⟩
+          else y
+        )
+    let last : Array (Range Char) :=
+      match interval.ranges.pop? with
+      | some (x, _) =>
+          if x.end < Bound.max_value
+          then #[⟨Bound.increment x.end, Bound.max_value, by
+              simp [Bound.increment_le_max_value x.end]
+            ⟩]
+          else #[]
+      | none => #[]
+
+    let ranges := ranges ++ last
+    canonicalize ranges
+
+/-- Intersection of interval sets -/
+def intersection (interval1 interval2 : IntervalSet Char) : IntervalSet Char :=
+  let ranges := intersection.loop 0 0 interval1.ranges interval2.ranges #[]
+  canonicalize ranges
+where
+  loop (a b : Nat) (ra rb acc : Array $ Range Char) : Array $ Range Char :=
+    if h₁ : a < ra.size then
+      if h₂ : b < rb.size then
+        let acc :=
+          match Range.intersection (ra.get ⟨a, h₁⟩) (rb.get ⟨b, h₂⟩) with
+          | some r => acc.push r
+          | none => acc
+
+        if (ra.get ⟨a, h₁⟩).end < (rb.get ⟨b, h₂⟩).end
+        then loop (a+1) b ra rb acc
+        else loop a (b+1) ra rb acc
+      else acc
+    else acc
+termination_by _ a b ra rb _ => (ra.size - a, rb.size - b)
+
+/-- Subtract the interval set `interval2` from `interval1`. -/
+def difference (interval1 interval2 : IntervalSet Char) : IntervalSet Char :=
+  intersection interval1 (negate interval2)
+
+/-- Union of interval sets. -/
+def union (interval1 interval2 : IntervalSet Char) : IntervalSet Char :=
+  if interval1.ranges.size = 0 then interval2
+  else if interval2.ranges.size = 0 then interval1
+  else canonicalize (interval1.ranges ++ interval2.ranges)
+
+/-- Compute the symmetric difference (A⊖B = (A∪B)\(A∩B)) of the two sets. -/
+def symmetric_difference (interval1 interval2 : IntervalSet Char) : IntervalSet Char :=
+  let intervalI := intersection interval1 interval2
+  let intervalU := union interval1 interval2
+  difference intervalU intervalI
