Regex/Interval/Lemmas.lean
@@ -1,0 +1,290 @@
+import Init.Data.Ord
+import Std.Logic
+import Std.Data.Nat.Lemmas
+import Std.Data.Fin.Lemmas
+import Std.Data.Int.Lemmas
+import Std.Data.List.Basic
+import Std.Data.Array.Init.Lemmas
+import Mathlib.Data.List.Chain
+import Regex.Utils
+import Regex.Bound
+import Regex.Data.UInt.Basic
+import Regex.Data.Char.Basic
+import Regex.Data.List.Lemmas
+import Regex.Data.Array.Basic
+import Regex.Data.Array.Lemmas
+import Regex.Interval.Basic
+
+namespace Ranges
+
+theorem empty_isNonOverlapping {α : Type u} [Ord α] [LT α] [LE α] [Bound α] [HSub α α Nat]
+    : nonOverlapping (#[] : Array (Range α)) := by
+  unfold nonOverlapping dataIsNonOverlapping
+  split <;> simp_all
+
+theorem single_isNonOverlapping (ranges : Array (Range Char)) (h : ranges.size = 1)
+    : nonOverlapping ranges  := by
+  unfold nonOverlapping dataIsNonOverlapping
+  split <;> try simp_all
+  unfold Array.size at h
+  unfold List.length at h
+  split at h <;> try simp_all
+  unfold List.length at h
+  split at h <;> try simp_all
+
+end Ranges
+
+instance (α : Type u) [Ord α] [LT α] [LE α] [Bound α] [HSub α α Nat]
+    [(a b : α) → Decidable (a < b)] [(a b : α) → Decidable (a = b)]
+    : Inhabited $ IntervalSet α where
+  default := ⟨#[], Ranges.empty_isNonOverlapping⟩
+
+namespace Interval
+
+def singleton (r : Range Char) : IntervalSet Char :=
+  let arr := #[r]
+  ⟨arr, by simp [Ranges.single_isNonOverlapping arr (Array.size_one r)]⟩
+
+theorem pred_lt' {n m : Nat} (h : m < n) : Nat.pred n < n :=
+  Nat.pred_lt (Nat.not_eq_zero_of_lt h)
+
+theorem Fin.pred {i : Fin n} (h : 0 < i.val) : LT.lt (i.val-1) n := by
+  have h1 : i.val-1 < i.val := pred_lt' h
+  have h2 : i.val < n := i.isLt
+  simp [Nat.lt_trans h1 h2]
+
+theorem isNonOverlapping (l r : Range Char)
+  (h1 : ¬(r.start.toNat - l.end.toNat) = 1) (h2 : ¬r.start < l.end) (h3 : ¬l.end = r.start)
+    : Range.nonOverlapping l r := by
+  have h1 : ¬1 = (r.start.toNat - l.end.toNat) := fun h => h1 (h.symm)
+  have h2 : l.end ≤  r.start := Nat.not_lt.mp h2
+  have h3 : ¬l.end.val.val = r.start.val.val := UInt32.val_ne_of_ne (Char.val_ne_of_ne h3)
+  have h : l.end.toNat < r.start.toNat := Nat.lt_of_le_of_ne h2 (Fin.val_ne_of_ne h3)
+  have h : l.end.toNat+1 ≤ r.start.toNat := Nat.succ_le_of_lt h
+  have h : 1 + l.end.toNat ≤ r.start.toNat := by rw [Nat.add_comm]; simp [h]
+  have h : 1 < r.start.toNat - l.end.toNat := Nat.lt_of_le_of_ne (Nat.le_sub_of_add_le h) h1
+  unfold Range.nonOverlapping
+  rw [← Range.Char.sub_def]
+  unfold Range.Char.sub
+  simp [h]
+
+theorem nonOverlappingWithLast_of_empty (ranges : Array $ Range Char) (next : Option (Range Char))
+    (h2 : ranges.size = 0) : nonOverlappingWithLast ranges next  := by
+  unfold nonOverlappingWithLast
+  split <;> try simp_all
+  · unfold Array.size List.length at h2
+    split at h2 <;> try simp_all
+    rename_i heq' x heq
+    unfold Array.last? at heq'
+    split at heq' <;> try simp_all
+    rename_i h
+    unfold List.length at h
+    split at h <;> try simp_all
+  · unfold Array.size List.length at h2
+    split at h2 <;> try simp_all
+    rename_i heq' x heq
+    unfold Array.last? at heq'
+    split at heq' <;> try simp_all
+    rename_i h
+    unfold List.length at h
+    split at h <;> try simp_all
+
+theorem nonOverlappingWithLast_with_none_eq_empty (acc : Acc) (h : acc.next.isNone)
+    : acc.set.ranges.size = 0 := by
+  have hx : nonOverlappingWithLast acc.set.ranges acc.next := acc.nonOverlapping
+  unfold nonOverlappingWithLast at hx
+  split at hx <;> try simp_all
+
+  rename_i heq _
+  unfold Array.last? at heq
+  split at heq <;> try simp_all
+
+theorem nonOverlappingWithLast_of_none (acc : Acc) (n : Range Char) (h : acc.next.isNone)
+    : nonOverlappingWithLast acc.set.ranges n  := by
+  have hx : acc.set.ranges.size = 0 := nonOverlappingWithLast_with_none_eq_empty acc h
+  simp [nonOverlappingWithLast_of_empty acc.set.ranges n hx]
+
+theorem nonOverlappingWithLast_of_val (acc : Acc) (n : Range Char) (h : is_start_eq acc.next n)
+    : nonOverlappingWithLast acc.set.ranges n  := by
+  have hx : nonOverlappingWithLast acc.set.ranges acc.next := acc.nonOverlapping
+  unfold nonOverlappingWithLast
+  unfold nonOverlappingWithLast at hx
+  unfold is_start_eq at h
+  simp_all
+  split <;> try simp_all
+  unfold Range.nonOverlapping
+  split at hx <;> try simp_all
+  unfold Range.nonOverlapping at hx
+  simp_all
+
+theorem is_start_eq_of_val (next : Option (Range Char)) (n: Range Char)
+  (hm : next = some l) (hx : l.start = n.start) : is_start_eq next n := by
+  unfold is_start_eq
+  simp_all
+
+theorem is_start_eq_of_none (next : Option (Range Char)) (n: Range Char)
+  (hm : next = none) : is_start_eq next n := by
+  unfold is_start_eq
+  simp_all
+
+theorem nonOverlappingWithLast_of_singleton (l r : Range Char) (h : Range.nonOverlapping l r)
+    : nonOverlappingWithLast (singleton l).ranges (some r)  := by
+  unfold singleton nonOverlappingWithLast
+  split <;> simp_all
+  unfold Range.nonOverlapping
+  rename_i heq _
+  unfold Array.last? at heq
+  split at heq <;> simp_all
+  unfold Range.nonOverlapping  at h
+  rename_i last' _ _ _
+  have heq' : List.get #[l].data ⟨0, by simp⟩ = l := List.singleton_val l (by simp)
+  simp_all
+
+theorem nonOverlapping_of_push (acc : Acc) (next : Range Char)
+  (h1: Array.last? acc.set.ranges = some last) (h2 : acc.next = some next)
+    : Ranges.nonOverlapping (Array.push acc.set.ranges next) := by
+  unfold Array.push Ranges.nonOverlapping
+  simp
+  have ⟨acc', hp⟩ := Array.pop?_of_last? acc.set.ranges h1
+  have h1 : acc.set.ranges.data = acc'.data ++ [last] := Array.concat_of_pop? hp
+  have h2 : Range.nonOverlapping last next := by
+    have hx : nonOverlappingWithLast acc.set.ranges acc.next := acc.nonOverlapping
+    unfold nonOverlappingWithLast at hx
+    split at hx <;> simp_all
+  have h5 : Ranges.dataIsNonOverlapping (acc'.data ++ [last] ++ [next]) := by
+    have hn : Ranges.nonOverlapping acc.set.ranges := acc.set.isNonOverlapping
+    unfold Ranges.nonOverlapping at hn
+    unfold Ranges.dataIsNonOverlapping
+    split <;> simp_all
+    rename_i heq
+    cases h : acc'.data
+    · rw [h] at heq
+      simp_all
+      rw [← heq.left, ← heq.right]
+      rw [← heq.left] at h2
+      have hx : List.Chain Range.nonOverlapping next [] := by simp_all
+      simp [List.chain_cons.mpr ⟨h2, hx⟩]
+      simp [h2]
+    · rw [h] at heq
+      rename_i head' tail' _ head tail
+      have hh : head = head' := List.head_eq_of_cons_eq heq
+      have ht : tail ++ [last] ++ [next] = tail' := by simp_all [List.tail_eq_of_cons_eq heq]
+      have hn : List.Chain Range.nonOverlapping head (tail ++ [last]) := by
+        unfold Ranges.dataIsNonOverlapping at hn
+        simp_all [hn]
+      have hy : List.Chain Range.nonOverlapping head (tail ++ [last]  ++ [next]) := by
+        simp [List.chain_append_cons_cons.mpr]
+        simp [h2]
+        simp [hn]
+      rw [←hh, ←ht]
+      simp_all [hy]
+  simp_all [h5]
+
+theorem List.eq_head_of_get_first (arr : List α) (h1 : 0 < arr.length)
+  (h2 : arr = head :: tail) : head = arr.get ⟨0, h1⟩ := by
+  cases arr
+  · contradiction
+  · unfold List.get
+    rename_i head' tail'
+    simp [List.head_eq_of_cons_eq h2]
+
+theorem Array.eq_head_of_get_first (arr : Array α) (h1 : 0 < arr.size)
+  (h2 : arr.data = head :: tail) : head = arr.get ⟨0, h1⟩ :=
+  List.eq_head_of_get_first arr.data h1 h2
+
+theorem List.eq_succ_of_tail_nth (arr : List α) (h1 : i+1 < arr.length)
+  (h2 : arr = head :: tail) (h3 : i < tail.length)
+    : tail.get ⟨i, h3⟩ = arr.get ⟨i+1, h1⟩ := by
+  cases h2
+  have h : (head :: tail).get ⟨i+1, h1⟩ = tail.get ⟨i, h3⟩ := List.get_cons_succ
+  exact h.symm
+
+theorem Array.eq_succ_of_tail_nth (arr : Array α) (h1 : i+1 < arr.size)
+  (h2 : arr.data = head :: tail) (h3 : i < tail.length)
+    : tail.get ⟨i, h3⟩ = arr.get ⟨i+1, h1⟩ :=
+  List.eq_succ_of_tail_nth arr.data h1 h2 h3
+
+theorem nonOverlapping_of_nth (ranges : Array $ Range Char) (n : Nat)
+  (h1 : 0 < n) (h2 : n+1 < Array.size ranges) (h3: ranges.data = head :: tail)
+  (h4 : ∀ (i : ℕ) (h : i < List.length tail-1),
+    Range.nonOverlapping (tail.get ⟨i, Nat.lt_of_lt_pred h⟩) (tail.get ⟨i+1, Nat.lt_pred_iff.mp h⟩))
+    : Range.nonOverlapping (ranges.get ⟨n, Nat.lt_of_succ_lt h2⟩) (ranges.get ⟨n+1, h2⟩) := by
+  have hlt : n < Array.size ranges := Nat.lt_of_succ_lt h2
+  have hf : n+1 < ranges.data.length := by unfold Array.size at h2; simp_all [h2]
+  have hne : ¬n = 0 := (Nat.ne_of_lt h1).symm
+  have hps : n-1+1 = n := Nat.succ_pred (by simp_all)
+  have ht0 : n < tail.length := by
+    have h : n < ranges.data.length-1 := Nat.pred_lt_pred (by simp [Nat.lt_of_le_of_ne]) hf
+    have h : n < tail.length := Nat.lt_of_lt_of_eq h (by simp_all)
+    simp [h]
+  have ht1 : n-1 < tail.length-1 := Nat.pred_lt_pred (by simp_all) ht0
+  have ht2 : n-1 < tail.length := Nat.lt_of_lt_pred ht1
+  have ht3 : n-1+1 < tail.length := by simp [hps, ht0]
+  have : Range.nonOverlapping (tail.get ⟨n-1, ht2⟩) (tail.get ⟨n-1+1, ht3⟩) := h4 (n-1) ht1
+  have : tail.get ⟨n-1, ht2⟩ = ranges.get ⟨n, hlt⟩ := by
+    let i := n-1
+    have h : i+1 < ranges.size := by simp [hps, hlt]
+    simp [Array.eq_succ_of_tail_nth ranges h h3 ht2]
+    simp [hps]
+  have : tail.get ⟨n-1+1, ht3⟩ = ranges.get ⟨n+1, hf⟩ := by
+    let i := n-1+1
+    have h : i < tail.length := by simp [hps, ht0]
+    simp [Array.eq_succ_of_tail_nth ranges (by simp [hps, hf]) h3 h]
+    simp [hps]
+  simp_all
+
+theorem nonOverlapping_of_pred (ranges : Array $ Range Char) (i : Fin (Array.size ranges))
+  (x y : Range Char) (h : 0 < i.val)
+  (hx : x = Array.get ranges ⟨i-1, Fin.pred h⟩) (hy : y = Array.get ranges i)
+  (hr : Ranges.nonOverlapping ranges)
+   : Range.nonOverlapping x y := by
+  unfold Ranges.nonOverlapping at hr
+  unfold Ranges.dataIsNonOverlapping at hr
+  split at hr <;> try simp_all
+  · rename_i heq
+    have : 0 = ranges.size := by unfold Array.size List.length; split <;> try simp_all
+    have : 0 ≠ ranges.size := by simp [Nat.ne_of_lt (Nat.lt_trans h i.isLt)]
+    contradiction
+  · rename_i heq
+    have : ¬1 < ranges.size := by unfold Array.size List.length; split <;> try simp_all
+    have : 1 < ranges.size := Nat.lt_of_le_of_lt (Nat.succ_le_of_lt h) i.isLt
+    contradiction
+  · rename_i head tail _ heq
+    let ⟨h1, h2⟩ := List.chain_iff_get.mp hr
+    match hm : i with
+    | ⟨0, h⟩ => contradiction
+    | ⟨1, hf⟩ =>
+      rename_i xt
+      have hx1 : 0 < ranges.size := by simp [Nat.lt_trans h hf]
+      have hx2 : 0 < tail.length := by cases tail <;> simp_all
+      have : Range.nonOverlapping head (List.get tail { val := 0, isLt := hx2}) := h1 hx2
+      have : head = ranges.get ⟨0, hx1⟩  := Array.eq_head_of_get_first ranges hx1 heq
+      have : tail.get ⟨0, hx2⟩  = ranges.get ⟨1, hf⟩ := Array.eq_succ_of_tail_nth ranges hf heq hx2
+      simp_all
+    | ⟨n+2, hf⟩ =>
+      have hx1 : n+1 < ranges.size := by simp [Nat.lt_trans _ hf]
+      have hx2 : Range.nonOverlapping ranges[n+1] ranges[n+2] :=
+        nonOverlapping_of_nth ranges (n+1) (by simp) hf heq h2
+      simp [hx2]
+
+theorem nonOverlappingWithLast_of_push(acc : Acc) (h1 : acc.next = some l)
+  (h2 : Ranges.nonOverlapping (Array.push acc.set.ranges l)) (h3 : Range.nonOverlapping l r)
+    : nonOverlappingWithLast (Acc.push acc l h2).ranges (some r) := by
+  unfold Acc.push Array.push nonOverlappingWithLast
+  split <;> try simp_all
+  rename_i last next heq _
+  unfold Array.last? at heq
+  split at heq <;> try simp_all
+  have hne : acc.set.ranges.data ++ [l] ≠ [] := by simp_all
+  have h : List.getLast (acc.set.ranges.data ++ [l]) hne
+      = List.get (acc.set.ranges.data ++ [l]) ⟨acc.set.ranges.data.length, (by simp_all)⟩ := by
+      have h : List.get (acc.set.ranges.data ++ [l]) ⟨acc.set.ranges.data.length, (by simp_all)⟩
+              = List.get (acc.set.ranges.data ++ [l])
+                  ⟨(acc.set.ranges.data ++ [l]).length-1, (by simp_all)⟩ := by
+        simp_all
+      rw [h]
+      rw [List.getLast_eq_get (acc.set.ranges.data ++ [l]) hne]
+  rw [← h] at heq
+  simp [List.getLast_append] at heq
+  rw [heq] at h3
+  simp [h3]
