lakefile.lean
@@ -2,13 +2,17 @@ import Lake
 open Lake DSL
 
 require UnicodeBasic from git "https://github.com/fgdorais/lean4-unicode-basic.git"
-   @  "main"
+   @  "8603bb1d0d5edae780e3a85a0398fd83dbbb80a3"
 
 require std from git "https://github.com/leanprover/std4"
-   @  "main"
+   @  "v4.5.0-rc1"
+
+require mathlib from git "https://github.com/leanprover-community/mathlib4"
+   @ "v4.5.0-rc1"
 
 meta if get_config? env = some "dev" then
-require «doc-gen4» from git "https://github.com/leanprover/doc-gen4" @ "main"
+require «doc-gen4» from git "https://github.com/leanprover/doc-gen4"
+   @ "94e10377bef4e64820ffd7dcab6affef3304af62"
 
 package «Regex» {
 }
